Provide syntactic sugar for examples

src/panRefinementExampleScript.sml
@@ -2,29 +2,43 @@ Theory panRefinementExample
 Ancestors panSem panRefinement
 Libs panRefinementLib
 
+Definition var_eq_def[simp]:
+  var_eq x (w : word64) = λs. FLOOKUP s.locals x = SOME (ValWord w)
+End
+
+Definition fixed_def[simp]:
+  fixed res = λr. res = r
+End
+
+Definition postcond_def[simp]:
+  postcond (qr : 'a result option -> bool)
+           (qt : ('a, 'ffi) state -> bool) = λ(r,t). qr r ∧ qt t
+End
+
+Definition var_word[simp]:
+  var_word x = λs. case FLOOKUP s.locals x of
+                   | SOME (ValWord w) => w
+                   | _                => 0w
+End
+
 Theorem assignment_1:
-  Abbrev (P = (λs. FLOOKUP s.locals x = SOME (ValWord 0w))) ∧
-  Abbrev (Q = (λ(r,s). r = NONE ∧ FLOOKUP s.locals x = SOME (ValWord 10w))) ∧
-  Abbrev (k = Local) ∧
-  Abbrev (src = (Const 10w)) ∧
-  Abbrev (v = x) ⇒
-  refine (HoareC P Q) (PanC (Assign k v src))
+  Abbrev (P = var_eq x 0w) ∧
+  Abbrev (Q = postcond (fixed NONE) (var_eq x 10w)) ⇒
+  refine (HoareC P Q) (PanC (Assign Local x (Const 10w)))
 Proof
   pan_refinement_tac assign_refinement_rule
 QED
 
 Theorem assignment_2_step_1:
-  Abbrev (P = (λs. FLOOKUP s.locals x = SOME (ValWord (0w : word64)))) ∧
-  Abbrev (Q = (λ(r,s). r = NONE ∧ FLOOKUP s.locals x = SOME (ValWord (10w : word64)))) ∧
+  Abbrev (P = var_eq x 0w) ∧
+  Abbrev (Q = postcond (fixed NONE) (var_eq x 10w)) ∧
   Abbrev (QB = (λs. F)) ∧
   Abbrev (QR = (λ(s,r). F)) ∧
   Abbrev (QE = (λ(s,eid,e). F)) ∧
   Abbrev (QF = (λ(s,f). F)) ∧
   Abbrev (e = (Cmp Less (Var Local x) (Const 10w))) ∧
-  Abbrev (v = (λs. case FLOOKUP s.locals x of
-                   | (SOME (ValWord w)) => w2n (11w - w)
-                   | _ => 0)) ∧
-  Abbrev (i = (λs. ∃w. FLOOKUP s.locals x = SOME (ValWord w) ∧ 0w ≤ w ∧ w ≤ 10w)) ⇒
+  Abbrev (v = (λs. w2n (11w - var_word x s))) ∧
+  Abbrev (i = (λs. ∃w. var_eq x w s ∧ 0w ≤ w ∧ w ≤ 10w)) ⇒
   refine (HoareC P Q)
          (WhileC e i v (HoareC (while_body_pre i e) (while_body_post i QB QR QE QF)))
 Proof
@@ -39,7 +53,7 @@ Theorem assignment_2_step_2:
   Abbrev (QE = (λ(s,eid,e). F)) ∧
   Abbrev (QF = (λ(s,f). F)) ∧
   Abbrev (e  = (Cmp Less (Var Local x) (Const 10w))) ∧
-  Abbrev (i = (λs. ∃w. FLOOKUP s.locals x = SOME (ValWord w) ∧ 0w ≤ w ∧ w ≤ (10w : word64))) ⇒
+  Abbrev (i = (λs. ∃w. var_eq x w s ∧ 0w ≤ w ∧ w ≤ 10w)) ⇒
   refine (HoareC P Q)
          (PanC (Assign Local x (Op Add [(Var Local x); (Const 1w)])))
 Proof
@@ -47,13 +61,11 @@ Proof
 QED
 
 Theorem assignment_2_step_3:
-  Abbrev (P = (λs. FLOOKUP s.locals x = SOME (ValWord (0w : word64)))) ∧
-  Abbrev (Q = (λ(r,s). r = NONE ∧ FLOOKUP s.locals x = SOME (ValWord (10w : word64)))) ∧
+  Abbrev (P = var_eq x 0w) ∧
+  Abbrev (Q = postcond (fixed NONE) (var_eq x 10w)) ∧
   Abbrev (e = (Cmp Less (Var Local x) (Const 10w))) ∧
-  Abbrev (v = (λs. case FLOOKUP s.locals x of
-                   | (SOME (ValWord w)) => w2n ((11w : word64) - w)
-                   | _ => 0)) ∧
-  Abbrev (i = (λs. ∃w. FLOOKUP s.locals x = SOME (ValWord w) ∧ 0w ≤ w ∧ w ≤ 10w)) ⇒
+  Abbrev (v = (λs. w2n (11w - var_word x s))) ∧
+  Abbrev (i = (λs. ∃w. var_eq x w s ∧ 0w ≤ w ∧ w ≤ 10w)) ⇒
   refine (WhileC e i v (PanC (Assign Local x (Op Add [(Var Local x); (Const 1w)]))))
          (PanC (While e (Assign Local x (Op Add [(Var Local x); (Const 1w)]))))
 Proof
